IdSimClight wip

driver/IdSimClight.v
@@ -18,6 +18,7 @@ Require Import LocationsC Conventions.
 
 Require Import AsmregsC.
 Require Import MatchSimModSem.
+Require Import ClightStep.
 
 Set Implicit Arguments.
 
@@ -78,6 +79,69 @@ Proof.
       * des_ifs.
 Qed.
 
+Lemma val_casted_injection val0 val1 j ty
+      (VAL: Val.inject j val0 val1)
+      (CAST: val_casted val0 ty)
+  :
+    val_casted val1 ty.
+Proof.
+  inv CAST; inv VAL; clarify; try econs; eauto.
+Qed.
+
+Require Import CtypingC.
+Require Import CopC.
+
+Lemma typecheck_injection vals0 vals1 j ty
+      (VALS: Val.inject_list j vals0 vals1)
+      (TYP: typecheck vals0 ty)
+  :
+    typecheck vals1 ty.
+Proof.
+  inv TYP. econs; eauto. clear - VALS TYP0.
+  revert vals1 VALS TYP0. generalize (typelist_to_listtype ty).
+  clear ty. induction vals0; ss.
+  - i. inv VALS. inv TYP0. econs.
+  - i. inv VALS. inv TYP0. econs.
+    + eapply val_casted_injection; eauto.
+    + eapply IHvals0; eauto.
+Qed.
+
+Lemma wt_retval_inject j v_src v_tgt ty
+      (INJ: Val.inject j v_src v_tgt)
+      (TYP: wt_retval v_tgt ty)
+  :
+    wt_retval v_src ty.
+Proof.
+  inv TYP; inv WTV; inv INJ; clarify; try by repeat (econs; eauto).
+  exploit NVOID; eauto. clarify.
+Qed.
+
+Lemma typify_c_injection j retv_src retv_tgt tres tv_src
+      (TYP: typify_c retv_src tres tv_src)
+      (INJ: Val.inject j retv_src retv_tgt)
+  :
+    exists tv_tgt,
+      (<<TYP: typify_c retv_tgt tres tv_tgt>>) /\
+      (<<INJ: Val.inject j tv_src tv_tgt>>).
+Proof.
+  inv TYP.
+  - destruct (classic (wt_retval retv_tgt tres)).
+    + esplits; eauto. econs; eauto.
+    + exists Vundef. esplits; eauto.
+      * econs 2. eauto.
+      * assert (tv_src = Vundef); clarify; eauto.
+        inv INJ; inv WT; inv WTV; clarify;
+          exfalso; eapply H; econs; clarify; try (econs; eauto).
+        exploit NVOID; eauto. clarify.
+  - exists Vundef. esplits; eauto.
+    econs 2. ii. exploit wt_retval_inject; eauto.
+Qed.
+
+Definition cgenv skenv_link clight :=
+  Build_genv
+    (SkEnv.revive (SkEnv.project skenv_link (CtypesC.CSk.of_program signature_of_function clight)) clight)
+    (prog_comp_env clight).
+
 Lemma clight1_inj_id
       (clight: Clight.program)
   :
@@ -87,148 +151,66 @@ Lemma clight1_inj_id
       /\ (<<TGT: mp.(ModPair.tgt) = clight.(module1)>>)
 .
 Proof.
-  admit "this should hold".
+  eexists (ModPair.mk _ _ _); s.
+  esplits; eauto. instantiate (1:=tt).
+  econs; ss; i.
+  eapply match_states_sim with (match_states := match_states_clight); ss.
+  - apply unit_ord_wf.
+  - eapply SoundTop.sound_state_local_preservation.
+
+  - i. ss.
+    inv INITTGT. inv SAFESRC. inv H. ss.
+    assert (FD: fd = fd0).
+    { admit "genv". } clarify.
+    esplits; eauto.
+    + econs; eauto.
+    + refl.
+    + inv SIMARGS. econs; eauto. econs.
+
+  - i. ss. des. inv SAFESRC. esplits. econs; ss.
+    + instantiate (1:=fd).
+      admit "genv".
+    + eapply typecheck_injection; eauto.
+      inv SIMARGS. ss. eauto.
+
+  - i. ss. inv MATCH; eauto.
+
+  - i. ss. clear SOUND. inv CALLSRC. inv MATCH. ss.
+    esplits; eauto.
+    + econs; ss; eauto.
+      * admit "genv".
+      * admit "genv".
+    + econs; ss.
+    + refl.
+    + instantiate (1:=top4). ss.
+
+  - i. ss. clear SOUND HISTORY.
+    exists (SimMemInj.unlift' sm_arg sm_ret).
+    inv AFTERSRC. inv MATCH.
+    exploit typify_c_injection; eauto.
+    { inv SIMRET; ss; eauto. } i. des.
+    esplits; eauto.
+    + econs; eauto.
+    + inv SIMRET. econs; eauto.
+      eapply match_cont_incr; cycle 1; eauto.
+      inv MLE. inv MLE0. ss. etrans; eauto.
+    + refl.
+
+  - i. ss. inv FINALSRC. inv MATCH. inv CONT.
+    esplits; eauto.
+    + econs.
+    + econs; eauto.
+    + refl.
+
+  - left. i. split.
+    + admit "receptive".
+    + ii. exploit clight_step_preserve_injection; try eassumption.
+      { instantiate (1:=cgenv skenv_link_tgt clight). ss. }
+      { eapply function_entry1_inject. ss. }
+      i. des. esplits; eauto.
+      left. apply plus_one. econs; ss; eauto.
+      admit "determinate".
 Qed.
-
-Definition match_env (j: meminj) (env_src env_tgt: env) :=
-  forall id,
-    (<<MAPPED: exists blk_src blk_tgt ty,
-        (<<INJ: j blk_src = Some (blk_tgt, 0)>>) /\
-        (<<BLKSRC: env_src ! id = Some (blk_src, ty)>>) /\
-        (<<BLKTGT: env_tgt ! id = Some (blk_tgt, ty)>>)>>) \/
-    (<<NOTMAPPED:
-       (<<BLKSRC: env_src ! id = None>>) /\
-       (<<BLKTGT: env_tgt ! id = None>>)>>)
-.
-
-Definition match_temp_env (j: meminj) (tenv_src tenv_tgt: temp_env) :=
-  forall id,
-    option_rel (Val.inject j) (tenv_src ! id) (tenv_tgt ! id).
-
-Inductive match_cont (j: meminj): cont -> cont -> Prop :=
-| match_Kstop:
-    match_cont j Kstop Kstop
-| match_Kseq
-    stmt K_src K_tgt
-    (CONT: match_cont j K_src K_tgt)
-  :
-    match_cont j (Kseq stmt K_src) (Kseq stmt K_tgt)
-| match_Kloop1
-    stmt0 stmt1 K_src K_tgt
-    (CONT: match_cont j K_src K_tgt)
-  :
-    match_cont j (Kloop1 stmt0 stmt1 K_src) (Kloop1 stmt0 stmt1 K_tgt)
-| match_Kloop2
-    stmt0 stmt1 K_src K_tgt
-    (CONT: match_cont j K_src K_tgt)
-  :
-    match_cont j (Kloop2 stmt0 stmt1 K_src) (Kloop2 stmt0 stmt1 K_tgt)
-| match_Kswitch
-    K_src K_tgt
-    (CONT: match_cont j K_src K_tgt)
-  :
-    match_cont j (Kswitch K_src) (Kswitch K_tgt)
-| match_Kcall
-    id fn
-    env_src env_tgt
-    tenv_src tenv_tgt
-    K_src K_tgt
-    (ENV: match_env j env_src env_tgt)
-    (TENV: match_temp_env j tenv_src tenv_tgt)
-    (CONT: match_cont j K_src K_tgt)
-  :
-    match_cont j (Kcall id fn env_src tenv_src K_src) (Kcall id fn env_tgt tenv_tgt K_tgt)
-.
-
-Inductive match_states_clight (sm_arg: SimMemInj.t')
-  : unit -> state -> state -> SimMemInj.t' -> Prop :=
-| match_State
-    fn stmt K_src K_tgt env_src env_tgt tenv_src tenv_tgt m_src m_tgt sm0
-    (MWFSRC: m_src = sm0.(SimMemInj.src))
-    (MWFTGT: m_tgt = sm0.(SimMemInj.tgt))
-    (MWF: SimMemInj.wf' sm0)
-    (ENV: match_env sm0.(SimMemInj.inj) env_src env_tgt)
-    (TENV: match_temp_env sm0.(SimMemInj.inj) tenv_src tenv_tgt)
-    (CONT: match_cont sm0.(SimMemInj.inj) K_src K_tgt)
-  :
-    match_states_clight
-      sm_arg tt
-      (State fn stmt K_src env_src tenv_src m_src)
-      (State fn stmt K_tgt env_tgt tenv_tgt m_tgt)
-      sm0
-| match_Callstate
-    fptr_src fptr_tgt ty args_src args_tgt K_src K_tgt m_src m_tgt sm0
-    (MWFSRC: m_src = sm0.(SimMemInj.src))
-    (MWFTGT: m_tgt = sm0.(SimMemInj.tgt))
-    (MWF: SimMemInj.wf' sm0)
-    (INJ: Val.inject sm0.(SimMemInj.inj) fptr_src fptr_tgt)
-    (VALS: Val.inject_list sm0.(SimMemInj.inj) args_src args_tgt)
-    (CONT: match_cont sm0.(SimMemInj.inj) K_src K_tgt)
-  :
-    match_states_clight
-      sm_arg tt
-      (Callstate fptr_src ty args_src K_src m_src)
-      (Callstate fptr_tgt ty args_tgt K_tgt m_tgt)
-      sm0
-| match_Returnstate
-    retv_src retv_tgt K_src K_tgt m_src m_tgt sm0
-    (MWFSRC: m_src = sm0.(SimMemInj.src))
-    (MWFTGT: m_tgt = sm0.(SimMemInj.tgt))
-    (MWF: SimMemInj.wf' sm0)
-    (INJ: Val.inject sm0.(SimMemInj.inj) retv_src retv_tgt)
-    (CONT: match_cont sm0.(SimMemInj.inj) K_src K_tgt)
-  :
-    match_states_clight
-      sm_arg tt
-      (Returnstate retv_src K_src m_src)
-      (Returnstate retv_tgt K_tgt m_tgt)
-      sm0
-.
-
-Inductive match_states_ext_clight (sm_arg: SimMemExt.t')
-  : unit -> state -> state -> SimMemExt.t' -> Prop :=
-| match_ext_State
-    fn stmt K_src K_tgt env_src env_tgt tenv_src tenv_tgt m_src m_tgt sm0
-    (MWFSRC: m_src = sm0.(SimMemExt.src))
-    (MWFTGT: m_tgt = sm0.(SimMemExt.tgt))
-    (MWF: Mem.extends m_src m_tgt)
-    (ENV: env_src = env_tgt)
-    (TENV: tenv_src = tenv_tgt)
-    (CONT: match_cont inject_id K_src K_tgt)
-  :
-    match_states_ext_clight
-      sm_arg tt
-      (State fn stmt K_src env_src tenv_src m_src)
-      (State fn stmt K_tgt env_tgt tenv_tgt m_tgt)
-      sm0
-| match_ext_Callstate
-    fptr_src fptr_tgt ty args_src args_tgt K_src K_tgt m_src m_tgt sm0
-    (MWFSRC: m_src = sm0.(SimMemExt.src))
-    (MWFTGT: m_tgt = sm0.(SimMemExt.tgt))
-    (MWF: Mem.extends m_src m_tgt)
-    (INJ: Val.lessdef fptr_src fptr_tgt)
-    (VALS: Val.lessdef_list args_src args_tgt)
-    (CONT: match_cont inject_id K_src K_tgt)
-  :
-    match_states_ext_clight
-      sm_arg tt
-      (Callstate fptr_src ty args_src K_src m_src)
-      (Callstate fptr_tgt ty args_tgt K_tgt m_tgt)
-      sm0
-| match_ext_Returnstate
-    retv_src retv_tgt K_src K_tgt m_src m_tgt sm0
-    (MWFSRC: m_src = sm0.(SimMemExt.src))
-    (MWFTGT: m_tgt = sm0.(SimMemExt.tgt))
-    (MWF: Mem.extends m_src m_tgt)
-    (INJ: Val.lessdef retv_src retv_tgt)
-    (CONT: match_cont inject_id K_src K_tgt)
-  :
-    match_states_ext_clight
-      sm_arg tt
-      (Returnstate retv_src K_src m_src)
-      (Returnstate retv_tgt K_tgt m_tgt)
-      sm0
-.
 
 Lemma clight2_id
       (clight: Clight.program)
@@ -324,754 +306,3 @@ Lemma clight2_inj_drop
 Proof.
   admit "this should hold".
 Qed.
-
-
-Require Import mktac.
-Require Import IntegersC.
-(* Require Import SimplLocalsproof. *)
-
-Section CLIGHTINJ.
-
-  Variable se_src se_tgt: Senv.t.
-  Variable ge_src ge_tgt: genv.
-  Hypothesis CENV: genv_cenv ge_src = genv_cenv ge_tgt.
-  (* TODO: injection condition of env *)
-
-  Definition function_entry_inject
-             (function_entry: genv -> function -> list val -> mem -> env -> temp_env -> mem -> Prop)
-    :=
-      forall
-        fn vs_src vs_tgt sm0 env_src tenv_src m_src1
-        (MWF: SimMemInj.wf' sm0)
-        (VALS: Val.inject_list sm0.(SimMemInj.inj) vs_src vs_tgt)
-        (ENTRY: function_entry ge_src fn vs_src sm0.(SimMemInj.src) env_src tenv_src m_src1),
-      exists env_tgt tenv_tgt sm1,
-        (<<MEMSRC: SimMemInj.src sm1 = m_src1>>) /\
-        (<<MWF: SimMemInj.wf' sm1>>) /\
-        (<<ENV: match_env sm1.(SimMemInj.inj) env_src env_tgt>>) /\
-        (<<TENV: match_temp_env sm1.(SimMemInj.inj) tenv_src tenv_tgt>>) /\
-        (<<MLE: SimMemInj.le' sm0 sm1>>) /\
-        (<<ENTRY: function_entry ge_tgt fn vs_tgt sm0.(SimMemInj.tgt) env_tgt tenv_tgt sm1.(SimMemInj.tgt)>>).
-
-  Lemma alloc_variables_inject sm0 idl e_src0 e_tgt0 e_src1 m_src1
-        (ALLOC: alloc_variables ge_src e_src0 (SimMemInj.src sm0) idl e_src1 m_src1)
-        (ENV: match_env (SimMemInj.inj sm0) e_src0 e_tgt0)
-        (MWF: SimMemInj.wf' sm0)
-    :
-      exists e_tgt1 sm1,
-        (<<MEMSRC: SimMemInj.src sm1 = m_src1>>) /\
-        (<<MWF: SimMemInj.wf' sm1>>) /\
-        (<<MLE: SimMemInj.le' sm0 sm1>>) /\
-        (<<ENV: match_env (SimMemInj.inj sm1) e_src1 e_tgt1>>) /\
-        (<<ALLOC: alloc_variables ge_tgt e_tgt0 (SimMemInj.tgt sm0) idl e_tgt1 (SimMemInj.tgt sm1)>>).
-  Proof.
-    revert sm0 MWF e_src0 e_tgt0 e_src1 m_src1 ENV ALLOC. induction idl.
-    - i. inv ALLOC. esplits; eauto.
-      + refl.
-      + econs.
-    - i. inv ALLOC.
-      exploit SimMemInj.alloc_parallel; eauto; try refl. i. des. clarify.
-      exploit IHidl; eauto.
-      { instantiate (1:=PTree.set id (blk_tgt, ty) e_tgt0).
-        ii. repeat rewrite PTree.gsspec. des_ifs.
-        - left. esplits; eauto.
-        - destruct (ENV id0).
-          + des. left. inv MLE. esplits; cycle 1; eauto.
-          + right. eauto. }
-      i. des. clarify.
-      esplits; eauto.
-      + etrans; eauto.
-      + econs; eauto.
-        rewrite <- CENV. auto.
-  Qed.
-
-  Lemma storebytes_mapped
-        sm0 b tb ofs bytes1 bytes2 m_src delta
-        (MWF : SimMemInj.wf' sm0)
-        (STRSRC: Mem.storebytes (SimMemInj.src sm0) b ofs bytes1 = Some m_src)
-        (SIMBLK: (SimMemInj.inj sm0) b = Some (tb, delta))
-        (BYTESINJ: list_forall2 (memval_inject (SimMemInj.inj sm0)) bytes1 bytes2)
-    (* (SIMADDR: Val.inject (SimMemInj.inj sm0) (Vptr b ofs) (Vptr tb tofs)) *)
-    :
-      exists sm1,
-        (<<MSRC: (SimMemInj.src sm1) = m_src>>)
-        /\ (<<MINJ: (SimMemInj.inj sm1) = (SimMemInj.inj sm0)>>)
-        /\ (<<STRTGT: Mem.storebytes (SimMemInj.tgt sm0) tb (ofs + delta) bytes2 = Some (SimMemInj.tgt sm1)>>)
-        /\ (<<MWF: SimMemInj.wf' sm1>>)
-        /\ (<<MLE: SimMemInj.le' sm0 sm1>>)
-  .
-  Proof.
-    (* inv SIMADDR. *)
-    exploit Mem.storebytes_mapped_inject; eauto.
-    { inv MWF. eauto. }
-    i. des.
-    inv MWF.
-    eexists (SimMemInj.mk _ _ _ _ _ _ _).
-    esplits; ss; eauto; cycle 1.
-    - econs; ss; eauto.
-      + eapply Mem.storebytes_unchanged_on; eauto.
-        ii. apply SRCEXT in H2. red in H2. des. red in H2. clarify.
-      + eapply Mem.storebytes_unchanged_on; eauto.
-        ii. apply TGTEXT in H2. red in H2. des. red in H2.
-        eapply H2; eauto. clear - BYTESINJ STRSRC H1 H4.
-        eapply Mem.storebytes_range_perm in STRSRC.
-        assert (Datatypes.length bytes2 = Datatypes.length bytes1).
-        { exploit list_forall2_length; eauto. }
-        rewrite H in *.
-        assert (ofs <= i - delta) by nia.
-        assert (i - delta < ofs + Z.of_nat (Datatypes.length bytes1)) by nia.
-        unfold Mem.range_perm in STRSRC.
-        specialize (STRSRC (i - delta)). exploit STRSRC. nia.
-        i. eapply Mem.perm_cur_max. eapply Mem.perm_implies; eauto.
-        eapply perm_any_N.
-      + eapply SimMemInj.frozen_refl.
-      + ii. eapply Mem.perm_storebytes_2; eauto.
-      + ii. eapply Mem.perm_storebytes_2; eauto.
-    - econs; ss; eauto.
-      + etransitivity; eauto. unfold SimMemInj.src_private. ss. ii; des. esplits; eauto.
-        unfold SimMemInj.valid_blocks in *. eauto with mem.
-      + etransitivity; eauto. unfold SimMemInj.tgt_private. ss. ii; des. esplits; eauto.
-        { ii. eapply PR. eauto with mem. eauto with mem. }
-        unfold SimMemInj.valid_blocks in *. eauto with mem.
-      + etransitivity; eauto. erewrite <- Mem.nextblock_storebytes; eauto. xomega.
-      + etransitivity; eauto. erewrite <- Mem.nextblock_storebytes; eauto. xomega.
-  Qed.
-
-  Lemma assign_loc_inject ce ty sm0 blk_src blk_tgt ofs_src ofs_tgt v_src v_tgt m_src1
-        (ASSIGN: assign_loc ce ty sm0.(SimMemInj.src) blk_src ofs_src v_src m_src1)
-        (INJ: Val.inject sm0.(SimMemInj.inj) (Vptr blk_src ofs_src) (Vptr blk_tgt ofs_tgt))
-        (VAL: Val.inject sm0.(SimMemInj.inj) v_src v_tgt)
-        (MWF: SimMemInj.wf' sm0)
-    :
-      exists sm1,
-        (<<ASSIGN: assign_loc ce ty sm0.(SimMemInj.tgt) blk_tgt ofs_tgt v_tgt sm1.(SimMemInj.tgt)>>) /\
-        (<<MEMSRC: SimMemInj.src sm1 = m_src1>>) /\
-        (<<MWF: SimMemInj.wf' sm1>>) /\
-        (<<MLE: SimMemInj.le' sm0 sm1>>).
-  Proof.
-    inv ASSIGN.
-    - exploit SimMemInj.storev_mapped; eauto. i. des.
-      esplits; eauto. econs 1; eauto.
-    - cinv MWF. cinv VAL. cinv INJ.
-      exploit Mem.loadbytes_inject; eauto. i. des_safe.
-      exploit storebytes_mapped; eauto. i. des_safe.
-      esplits; eauto. admit "TODO".
-  Qed.
-
-  Lemma call_cont_match j K_src K_tgt
-        (MATCH: match_cont j K_src K_tgt)
-    :
-      match_cont j (call_cont K_src) (call_cont K_tgt).
-  Proof.
-    revert K_tgt MATCH. induction K_src; ss; i; inv MATCH; ss; eauto.
-    - econs.
-    - econs; eauto.
-  Qed.
-
-  Lemma match_env_incr j0 j1
-        (INCR: inject_incr j0 j1)
-    :
-      match_env j0 <2= match_env j1.
-  Proof.
-    ii. destruct (PR id).
-    - des. left. esplits; eauto.
-    - des. right. esplits; eauto.
-  Qed.
-
-  Lemma match_temp_env_incr j0 j1
-        (INCR: inject_incr j0 j1)
-    :
-      match_temp_env j0 <2= match_temp_env j1.
-  Proof.
-    ii. destruct (PR id); econs. eapply val_inject_incr; eauto.
-  Qed.
-
-  Lemma match_cont_incr j0 j1
-        (INCR: inject_incr j0 j1)
-    :
-      match_cont j0 <2= match_cont j1.
-  Proof.
-    ii. revert INCR.
-    induction PR; i; econs; eauto; try by (eapply match_expr_incr; eauto).
-    - eapply match_env_incr; eauto.
-    - eapply match_temp_env_incr; eauto.
-  Qed.
-
-  Lemma bind_parameters_inject e_src e_tgt sm0 idl vargs_src vargs_tgt m_src1
-        (BIND: bind_parameters ge_src e_src (SimMemInj.src sm0) idl vargs_src m_src1)
-        (ENV: match_env (SimMemInj.inj sm0) e_src e_tgt)
-        (MWF: SimMemInj.wf' sm0)
-        (VALS: Val.inject_list (SimMemInj.inj sm0) vargs_src vargs_tgt)
-    :
-      exists sm1,
-        (<<MEMSRC: SimMemInj.src sm1 = m_src1>>) /\
-        (<<MWF: SimMemInj.wf' sm1>>) /\
-        (<<MLE: SimMemInj.le' sm0 sm1>>) /\
-        (<<BIND: bind_parameters ge_tgt e_tgt (SimMemInj.tgt sm0) idl vargs_tgt (SimMemInj.tgt sm1)>>).
-  Proof.
-    revert sm0 ENV vargs_src vargs_tgt m_src1 MWF VALS BIND. induction idl.
-    - i. inv BIND. inv VALS. esplits; eauto.
-      + refl.
-      + econs.
-    - i. inv BIND. inv VALS.
-      destruct (ENV id); des; clarify.
-      exploit assign_loc_inject; eauto. i. des. clarify.
-      exploit IHidl; try apply H6; eauto.
-      { inv MLE. eapply match_env_incr; eauto. }
-      { inv MLE. eapply val_inject_list_incr; eauto. }
-      i. des. esplits; eauto.
-      + etrans; eauto.
-      + econs; eauto. rewrite CENV in *. auto.
-  Qed.
-
-  Lemma set_match_temp_env j id v_src v_tgt tenv_src tenv_tgt
-        (TENV: match_temp_env j tenv_src tenv_tgt)
-        (VAL: Val.inject j v_src v_tgt)
-    :
-      match_temp_env j (PTree.set id v_src tenv_src) (PTree.set id v_tgt tenv_tgt).
-  Proof.
-    ii. repeat rewrite PTree.gsspec. des_ifs.
-    econs; eauto.
-  Qed.
-
-  Lemma bind_parameter_temps_inject tenv_src0 tenv_tgt0 tenv_src1
-        j idl vargs_src vargs_tgt
-        (BIND: bind_parameter_temps idl vargs_src tenv_src0 = Some tenv_src1)
-        (TENV: match_temp_env j tenv_src0 tenv_tgt0)
-        (VALS: Val.inject_list j vargs_src vargs_tgt)
-    :
-      exists tenv_tgt1,
-        (<<BIND: bind_parameter_temps idl vargs_tgt tenv_tgt0 = Some tenv_tgt1>>) /\
-        (<<TENV: match_temp_env j tenv_src1 tenv_tgt1>>).
-  Proof.
-    revert tenv_src0 tenv_tgt0 tenv_src1 vargs_src BIND TENV vargs_tgt VALS.
-    induction idl; i; ss; des_ifs_safe.
-    - inv VALS. esplits; eauto.
-    - inv VALS. exploit IHidl; eauto.
-      eapply set_match_temp_env; eauto.
-  Qed.
-
-  Lemma create_undef_temps_match j l
-    :
-      match_temp_env j (create_undef_temps l) (create_undef_temps l).
-  Proof.
-    induction l; ss.
-    - ii. repeat rewrite PTree.gempty. econs.
-    - ii. des_ifs. rewrite PTree.gsspec.
-      des_ifs. econs. eauto.
-  Qed.
-
-  Lemma function_entry1_inject
-    :
-      function_entry_inject function_entry1.
-  Proof.
-    ii. inv ENTRY.
-    exploit alloc_variables_inject; eauto.
-    { instantiate (1:=empty_env). ii. right.
-      unfold empty_env. repeat rewrite PTree.gempty. auto. }
-    i. des. clarify.
-    exploit bind_parameters_inject; eauto.
-    { cinv MLE. eapply val_inject_list_incr; eauto. } i. des.
-    esplits; eauto.
-    - cinv MLE. cinv MLE0. eapply match_env_incr; eauto.
-    - eapply create_undef_temps_match.
-    - etrans; eauto.
-    - econs; eauto.
-  Qed.
-
-  Lemma function_entry2_inject
-    :
-      function_entry_inject function_entry2.
-  Proof.
-    ii. inv ENTRY.
-    exploit alloc_variables_inject; eauto.
-    { instantiate (1:=empty_env). ii. right.
-      unfold empty_env. repeat rewrite PTree.gempty. auto. }
-    i. des. clarify.
-    exploit bind_parameter_temps_inject; eauto.
-    { eapply create_undef_temps_match. } i. des.
-    esplits; eauto.
-    - cinv MLE. eapply match_temp_env_incr; eauto.
-    - econs; eauto.
-  Qed.
-
-  Variable function_entry: genv -> function -> list val -> mem -> env -> temp_env -> mem -> Prop.
-  Hypothesis FUNCTIONENTRY: function_entry_inject function_entry.
-
-  Lemma deref_loc_inject j ty m_src m_tgt blk_src blk_tgt ofs_src ofs_tgt v_src
-        (DEREF: deref_loc ty m_src blk_src ofs_src v_src)
-        (INJECT: Mem.inject j m_src m_tgt)
-        (VAL: Val.inject j (Vptr blk_src ofs_src) (Vptr blk_tgt ofs_tgt))
-    :
-      exists v_tgt,
-        (<<DEREF: deref_loc ty m_tgt blk_tgt ofs_tgt v_tgt>>) /\
-        (<<VAL: Val.inject j v_src v_tgt>>).
-  Proof.
-    inv DEREF.
-    - exploit Mem.loadv_inject; eauto. i. des.
-      esplits; eauto. econs 1; eauto.
-    - esplits; eauto. econs 2; eauto.
-    - esplits; eauto. econs 3; eauto.
-  Qed.
-
-  Lemma eval_expr_lvalue_inject j env_src env_tgt tenv_src tenv_tgt m_src m_tgt
-    :
-      (forall
-          exp v_src
-          (EVAL: eval_expr ge_src env_src tenv_src m_src exp v_src),
-          forall
-            (ENV: match_env j env_src env_tgt)
-            (TENV: match_temp_env j tenv_src tenv_tgt)
-            (INJECT: Mem.inject j m_src m_tgt),
-          exists v_tgt,
-            (<<EVAL: eval_expr ge_tgt env_tgt tenv_tgt m_tgt exp v_tgt>>) /\
-            (<<INJ: Val.inject j v_src v_tgt>>)) /\
-      (forall
-          exp blk_src ofs_src
-          (EVAL: eval_lvalue ge_src env_src tenv_src m_src exp blk_src ofs_src),
-          forall
-            (ENV: match_env j env_src env_tgt)
-            (TENV: match_temp_env j tenv_src tenv_tgt)
-            (INJECT: Mem.inject j m_src m_tgt),
-          exists blk_tgt ofs_tgt,
-            (<<EVAL: eval_lvalue ge_tgt env_tgt tenv_tgt m_tgt exp blk_tgt ofs_tgt>>) /\
-            (<<INJ: Val.inject j (Vptr blk_src ofs_src) (Vptr blk_tgt ofs_tgt)>>)).
-  Proof.
-    apply eval_expr_lvalue_ind; i.
-    - esplits; eauto. econs 1; eauto.
-    - esplits; eauto. econs 2; eauto.
-    - esplits; eauto. econs 3; eauto.
-    - esplits; eauto. econs 4; eauto.
-    - cinv (TENV id); rewrite H in *; clarify.
-      esplits; eauto. econs 5; eauto.
-    - exploit H0; eauto. i. des.
-      esplits; eauto. econs 6; eauto.
-    - exploit H0; eauto. i. des.
-      exploit sem_unary_operation_inject; eauto. i. des.
-      esplits; eauto. econs 7; eauto.
-    - exploit H0; eauto. i. des.
-      exploit H2; eauto. i. des.
-      exploit sem_binary_operation_inject; eauto. i. des.
-      esplits; eauto. econs 8; eauto.
-      rewrite <- CENV. auto.
-    - exploit H0; eauto. i. des.
-      exploit sem_cast_inject; eauto. i. des.
-      esplits; eauto. econs 9; eauto.
-    - esplits; eauto. rewrite CENV. econs 10; eauto.
-    - esplits; eauto. rewrite CENV. econs 11; eauto.
-    - exploit H0; eauto. i. des.
-      exploit deref_loc_inject; eauto. i. des.
-      esplits; eauto. econs 12; eauto.
-    - cinv (ENV id); des; rewrite H in *; clarify.
-      esplits; eauto. econs 1; eauto.
-    - cinv (ENV id); des; rewrite H in *; clarify.
-      admit "genv".
-    - exploit H0; eauto. i. des. cinv INJ.
-      esplits; eauto. econs 3; eauto.
-    - exploit H0; eauto. i. des. cinv INJ. rewrite CENV in *.
-      esplits.
-      + econs 4; eauto.
-      + econs; eauto.
-        repeat rewrite Ptrofs.add_assoc. f_equal.
-        apply Ptrofs.add_commut.
-    - exploit H0; eauto. i. des. cinv INJ. rewrite CENV in *.
-      esplits; eauto. econs 5; eauto.
-  Qed.
-
-  Lemma eval_expr_inject j env_src env_tgt tenv_src tenv_tgt m_src m_tgt
-        exp v_src
-        (EVAL: eval_expr ge_src env_src tenv_src m_src exp v_src)
-        (ENV: match_env j env_src env_tgt)
-        (TENV: match_temp_env j tenv_src tenv_tgt)
-        (INJECT: Mem.inject j m_src m_tgt)
-    :
-      exists v_tgt,
-        (<<EVAL: eval_expr ge_tgt env_tgt tenv_tgt m_tgt exp v_tgt>>) /\
-        (<<INJ: Val.inject j v_src v_tgt>>).
-  Proof.
-    exploit eval_expr_lvalue_inject; eauto. i. des. eauto.
-  Qed.
-
-  Lemma eval_exprlist_inject j env_src env_tgt tenv_src tenv_tgt m_src m_tgt tys
-        exps vs_src
-        (EVALS: eval_exprlist ge_src env_src tenv_src m_src exps tys vs_src)
-        (ENV: match_env j env_src env_tgt)
-        (TENV: match_temp_env j tenv_src tenv_tgt)
-        (INJECT: Mem.inject j m_src m_tgt)
-    :
-      exists vs_tgt,
-        (<<EVALS: eval_exprlist ge_tgt env_tgt tenv_tgt m_tgt exps tys vs_tgt>>) /\
-        (<<INJ: Val.inject_list j vs_src vs_tgt>>).
-  Proof.
-    revert tys vs_src EVALS ENV TENV INJECT. induction exps; i.
-    - inv EVALS. exists []. esplits; eauto. econs; eauto.
-    - inv EVALS. exploit IHexps; eauto. i. des.
-      exploit eval_expr_inject; eauto. i. des.
-      exploit sem_cast_inject; eauto. i. des.
-      exists (tv :: vs_tgt). esplits; eauto.
-      econs; eauto.
-  Qed.
-
-  Lemma eval_lvalue_inject j env_src env_tgt tenv_src tenv_tgt m_src m_tgt
-        exp blk_src ofs_src
-        (EVAL: eval_lvalue ge_src env_src tenv_src m_src exp blk_src ofs_src)
-        (ENV: match_env j env_src env_tgt)
-        (TENV: match_temp_env j tenv_src tenv_tgt)
-        (INJECT: Mem.inject j m_src m_tgt)
-    :
-      exists blk_tgt ofs_tgt,
-        (<<EVAL: eval_lvalue ge_tgt env_tgt tenv_tgt m_tgt exp blk_tgt ofs_tgt>>) /\
-        (<<INJ: Val.inject j (Vptr blk_src ofs_src) (Vptr blk_tgt ofs_tgt)>>).
-  Proof.
-    exploit eval_expr_lvalue_inject; eauto. i. des. eauto.
-  Qed.
-
-  Definition match_loc j (loc_src loc_tgt: block * Z * Z): Prop :=
-    match loc_src with
-    | (blk_src, lo_src, hi_src) =>
-      match loc_tgt with
-      | (blk_tgt, lo_tgt, hi_tgt) =>
-        exists delta,
-        (<<DELTA: j blk_src = Some (blk_tgt, delta)>>) /\
-        (<<LO: lo_src + delta = lo_tgt>>) /\
-        (<<HI: hi_src + delta = hi_tgt>>)
-      end
-    end.
-
-  Lemma free_list_parallel
-        sm0 locs_src locs_tgt m_src1
-        (MWF: SimMemInj.wf' sm0)
-        (LOCS: list_forall2 (match_loc (SimMemInj.inj sm0)) locs_src locs_tgt)
-        (FREE: Mem.free_list (SimMemInj.src sm0) locs_src = Some m_src1)
-    :
-      exists sm1,
-        (<<MEMSRC: SimMemInj.src sm1 = m_src1>>) /\
-        (<<MWF: SimMemInj.wf' sm1>>) /\
-        (<<MLE: SimMemInj.le' sm0 sm1>>) /\
-        (<<FREE: Mem.free_list (SimMemInj.tgt sm0) locs_tgt = Some (SimMemInj.tgt sm1)>>).
-  Proof.
-    revert sm0 locs_tgt m_src1 MWF LOCS FREE. induction locs_src; ss.
-    - i. clarify. inv LOCS. esplits; eauto. refl.
-    - i. inv LOCS. unfold match_loc in H1. des_ifs. des. clarify. ss.
-      exploit SimMemInj.free_parallel; eauto. i. des. clarify.
-      exploit IHlocs_src; eauto.
-      { eapply list_forall2_imply; eauto. i. unfold match_loc in *. des_ifs.
-        des. inv MLE. esplits; eauto. }
-      i. des. clarify.
-      esplits; eauto.
-      + etrans; eauto.
-      + ss. rewrite FREETGT. eauto.
-  Qed.
-
-  Lemma blocks_of_env_match j e_src e_tgt
-        (ENV: match_env j e_src e_tgt)
-    :
-      list_forall2 (match_loc j) (blocks_of_env ge_src e_src) (blocks_of_env ge_tgt e_tgt).
-  Proof.
-    set (R:=(fun (d_src d_tgt: block * type) =>
-               let (b_src, t_src) := d_src in
-               let (b_tgt, t_tgt) := d_tgt in
-               (<<INJ: j b_src = Some (b_tgt, 0)>>) /\
-               (<<TYSAME: t_src = t_tgt>>))).
-    exploit PTree.elements_canonical_order.
-    - instantiate (1:=R).
-      instantiate (1:=e_tgt).
-      instantiate (1:=e_src).
-      i. destruct (ENV i); des; clarify.
-      esplits; eauto. ss.
-    - i. destruct (ENV i); des; clarify.
-      esplits; eauto. ss.
-    - intros ALL.
-      unfold blocks_of_env. revert ALL.
-      generalize (PTree.elements e_tgt).
-      generalize (PTree.elements e_src).
-      induction l; ss; i.
-      + inv ALL. econs.
-      + inv ALL. ss. econs; eauto.
-        unfold block_of_binding. des_ifs; ss; des; clarify.
-        esplits; eauto.
-        rewrite CENV. zsimpl. auto.
-  Qed.
-
-  Scheme statement_ind2 := Induction for statement Sort Prop
-    with labeled_statements_ind2 := Induction for labeled_statements Sort Prop.
-  Combined Scheme statement_labeled_statements_ind from statement_ind2, labeled_statements_ind2.
-
-  Lemma find_label_label_ls_match_none j lbl
-    :
-      (forall stmt,
-          forall K_src0 K_tgt0
-                 (LABEL: find_label lbl stmt K_src0 = None)
-                 (CONT: match_cont j K_src0 K_tgt0),
-            find_label lbl stmt K_tgt0 = None) /\
-      (forall ls,
-          forall K_src0 K_tgt0
-                 (LABEL: find_label_ls lbl ls K_src0 = None)
-                 (CONT: match_cont j K_src0 K_tgt0),
-            find_label_ls lbl ls K_tgt0 = None).
-  Proof.
-    eapply statement_labeled_statements_ind; ss; i.
-    - des_ifs_safe. exploit H; eauto.
-      { econs; eauto. } intros LABEL0.
-      rewrite LABEL0. eauto.
-    - des_ifs_safe. exploit H; eauto. intros LABEL0.
-      exploit H0; eauto. intros LABEL1.
-      rewrite LABEL0. eauto.
-    - des_ifs_safe. exploit H; eauto.
-      { econs; eauto. } intros LABEL0.
-      exploit H0; eauto.
-      { econs; eauto. } intros LABEL1.
-      rewrite LABEL0. eauto.
-    - exploit H; eauto. econs; eauto.
-    - des_ifs. exploit H; eauto.
-    - des_ifs_safe. exploit H; eauto.
-      { econs; eauto. } intros LABEL0.
-      rewrite LABEL0.
-      exploit H0; eauto.
-  Qed.
-
-  Lemma find_label_match_none j lbl stmt K_src0 K_tgt0
-        (LABEL: find_label lbl stmt K_src0 = None)
-        (CONT: match_cont j K_src0 K_tgt0)
-    :
-      find_label lbl stmt K_tgt0 = None.
-  Proof.
-    eapply find_label_label_ls_match_none; eauto.
-  Qed.
-
-  Lemma find_label_label_ls_match j lbl
-    :
-      (forall
-          stmt K_src0 K_tgt0 stmt' K_src1
-          (LABEL: find_label lbl stmt K_src0 = Some (stmt', K_src1))
-          (CONT: match_cont j K_src0 K_tgt0),
-          exists K_tgt1,
-            (<<LABEL: find_label lbl stmt K_tgt0 = Some (stmt', K_tgt1)>>) /\
-            (<<CONT: match_cont j K_src1 K_tgt1>>)) /\
-      (forall
-          ls K_src0 K_tgt0 stmt' K_src1
-          (LABEL: find_label_ls lbl ls K_src0 = Some (stmt', K_src1))
-          (CONT: match_cont j K_src0 K_tgt0),
-          exists K_tgt1,
-            (<<LABEL: find_label_ls lbl ls K_tgt0 = Some (stmt', K_tgt1)>>) /\
-            (<<CONT: match_cont j K_src1 K_tgt1>>)).
-  Proof.
-    eapply statement_labeled_statements_ind; ss; i.
-    - destruct (find_label lbl s (Kseq s0 K_src0)) eqn:LABEL0.
-      + clarify. exploit H; eauto.
-        { econs; eauto. } i. des.
-        rewrite LABEL. esplits; eauto.
-      + exploit H0; eauto. i. des.
-        exploit find_label_match_none; eauto.
-        { econs; eauto. } intros LABEL2.
-        rewrite LABEL1. rewrite LABEL2. esplits; eauto.
-    - destruct (find_label lbl s K_src0) eqn:LABEL0.
-      + clarify. exploit H; eauto. i. des.
-        rewrite LABEL. esplits; eauto.
-      + exploit find_label_match_none; eauto.
-        intros LABEL1. rewrite LABEL1.
-        exploit H0; eauto.
-    - destruct (find_label lbl s (Kloop1 s s0 K_src0)) eqn:LABEL0.
-      + clarify. exploit H; eauto.
-        { econs; eauto. } i. des.
-        rewrite LABEL. esplits; eauto.
-      + exploit find_label_match_none; eauto.
-        { econs; eauto. }
-        intros LABEL1. rewrite LABEL1.
-        exploit H0; eauto.
-        econs; eauto.
-    - exploit H; eauto.
-      econs; eauto.
-    - des_ifs.
-      + esplits; eauto.
-      + exploit H; eauto.
-    - destruct (find_label lbl s (Kseq (seq_of_labeled_statement l) K_src0)) eqn:LABEL0.
-      + clarify. exploit H; eauto.
-        { econs; eauto. } i. des.
-        rewrite LABEL. esplits; eauto.
-      + exploit find_label_match_none; eauto.
-        { econs; eauto. }
-        intros LABEL1. rewrite LABEL1.
-        exploit H0; eauto.
-  Qed.
-
-  Lemma find_label_match j lbl stmt K_src0 K_tgt0 stmt' K_src1
-        (LABEL: find_label lbl stmt K_src0 = Some (stmt', K_src1))
-        (CONT: match_cont j K_src0 K_tgt0)
-    :
-      exists K_tgt1,
-        (<<LABEL: find_label lbl stmt K_tgt0 = Some (stmt', K_tgt1)>>) /\
-        (<<CONT: match_cont j K_src1 K_tgt1>>)
-  .
-  Proof.
-    eapply find_label_label_ls_match; eauto.
-  Qed.
-
-  Lemma clight_step_preserve_injection
-        sm_arg u st_src0 st_tgt0 st_src1 sm0 tr
-        (MATCH: match_states_clight sm_arg u st_src0 st_tgt0 sm0)
-        (STEP: step se_src ge_src (function_entry ge_src) st_src0 tr st_src1)
-    :
-      exists st_tgt1 sm1,
-        (<<STEP: step se_tgt ge_tgt (function_entry ge_tgt) st_tgt0 tr st_tgt1>>) /\
-        (<<MATCH: match_states_clight sm_arg u st_src1 st_tgt1 sm1>>) /\
-        (<<MLE: SimMemInj.le' sm0 sm1>>).
-  Proof.
-    inv STEP; inv MATCH.
-    - cinv MWF. exploit eval_expr_inject; eauto. i. des.
-      exploit eval_lvalue_inject; eauto. i. des.
-      exploit sem_cast_inject; eauto. i. des.
-      exploit assign_loc_inject; eauto. i. des.
-      rewrite CENV in *.
-      esplits.
-      + econs 1; eauto.
-      + cinv MLE. econs; eauto.
-        * eapply match_env_incr; eauto.
-        * eapply match_temp_env_incr; eauto.
-        * eapply match_cont_incr; eauto.
-      + eauto.
-
-    - cinv MWF. exploit eval_expr_inject; eauto. i. des. esplits.
-      + econs 2; eauto.
-      + econs; eauto.
-        eapply set_match_temp_env; eauto.
-      + refl.
-
-    - cinv MWF. exploit eval_exprlist_inject; eauto. i. des.
-      exploit eval_expr_inject; eauto. i. des. esplits.
-      + econs 3; eauto.
-      + econs; eauto. econs; eauto.
-      + refl.
-
-    - cinv MWF. exploit eval_exprlist_inject; eauto. i. des.
-      admit "external call".
-
-    - esplits.
-      + econs 5; eauto.
-      + econs; eauto. econs; eauto.
-      + refl.
-
-    - inv CONT. esplits.
-      + econs 6; eauto.
-      + econs; eauto.
-      + refl.
-
-    - inv CONT. esplits.
-      + econs 7; eauto.
-      + econs; eauto.
-      + refl.
-
-    - inv CONT. esplits.
-      + econs 8; eauto.
-      + econs; eauto.
-      + refl.
-
-    - cinv MWF. exploit eval_expr_inject; eauto. i. des.
-      exploit bool_val_inject; eauto. i. esplits.
-      + econs 9; eauto.
-      + econs; eauto.
-      + refl.
-
-    - esplits.
-      + econs 10; eauto.
-      + econs; eauto. econs; eauto.
-      + refl.
-
-    - inv CONT. esplits.
-      + econs 11; eauto.
-      + econs; eauto. econs; eauto.
-      + refl.
-
-    - inv CONT. esplits.
-      + econs 12; eauto.
-      + econs; eauto.
-      + refl.
-
-    - inv CONT. esplits.
-      + econs 13; eauto.
-      + econs; eauto.
-      + refl.
-
-    - inv CONT. esplits.
-      + econs 14; eauto.
-      + econs; eauto.
-      + refl.
-
-    - exploit free_list_parallel; eauto.
-      { eapply blocks_of_env_match; eauto. } i. des.
-      esplits.
-      + econs 15; eauto.
-      + econs; eauto. eapply call_cont_match; eauto.
-        cinv MLE. eapply match_cont_incr; eauto.
-      + eauto.
-
-    - cinv MWF. exploit eval_expr_inject; eauto. i. des.
-      exploit sem_cast_inject; eauto. i. des.
-      exploit free_list_parallel; eauto.
-      { eapply blocks_of_env_match; eauto. } i. des.
-      esplits.
-      + econs 16; eauto.
-      + econs; eauto.
-        * cinv MLE. eapply val_inject_incr; eauto.
-        * eapply call_cont_match; eauto.
-          cinv MLE. eapply match_cont_incr; eauto.
-      + eauto.
-
-    - cinv MWF. exploit free_list_parallel; eauto.
-      { eapply blocks_of_env_match; eauto. } i. des.
-      esplits.
-      + econs 17; eauto.
-        unfold is_call_cont in *. destruct CONT; clarify.
-      + econs; eauto.
-        cinv MLE. eapply match_cont_incr; eauto.
-      + eauto.
-
-    - cinv MWF. exploit eval_expr_inject; eauto. i. des.
-      assert (SWITCH: sem_switch_arg v_tgt (typeof a) = Some n).
-      { unfold sem_switch_arg in *. inv INJ; ss; clarify; des_ifs. }
-      esplits.
-      + econs 18; eauto.
-      + econs; eauto. econs; eauto.
-      + refl.
-
-    - inv CONT. esplits.
-      + econs 19; eauto.
-      + econs; eauto.
-      + refl.
-
-    - inv CONT. esplits.
-      + econs 20; eauto.
-      + econs; eauto.
-      + refl.
-
-    - esplits.
-      + econs 21; eauto.
-      + econs; eauto.
-      + refl.
-
-    - exploit find_label_match; eauto.
-      { eapply call_cont_match; eauto. } i. des.
-      esplits.
-      + econs 22; eauto.
-      + econs; eauto.
-      + refl.
-
-    - assert (FPTRTGT: Genv.find_funct ge_tgt fptr_tgt = Some (Internal f)).
-      { admit "genv". }
-      exploit FUNCTIONENTRY; eauto. i. des.
-      esplits.
-      + econs 23; eauto.
-      + econs; eauto.
-        cinv MLE. eapply match_cont_incr; eauto.
-      + eauto.
-
-    - assert (FPTRTGT: Genv.find_funct ge_tgt fptr_tgt = Some (External ef targs tres cconv)).
-      { admit "genv". }
-      admit "external_call".
-
-    - inv CONT. esplits.
-      + econs 25; eauto.
-      + econs; eauto. destruct optid; ss.
-        eapply set_match_temp_env; eauto.
-      + refl.
-  Qed.
